\input{config.tex}
\begin{document} 

\begin{multicols}{5}
\setlength{\premulticols}{1pt}
\setlength{\postmulticols}{1pt}
\setlength{\multicolsep}{1pt}
\setlength{\columnsep}{2pt}

\section{Simplified Masters}
\begin{align*}
	T(n) &= aT(\frac{n}{b})+\Theta(n^d) \\
	a &\geq 1 \\
	b &> 1 \\
	d &\geq 0
\end{align*}
\begin{itemize}
	\item $a > b^d \rightarrow T(n) = \Theta(n^{\log_ba})$
	\item $a = b^d \rightarrow T(n) = \Theta(n^d\log_bn)$
	\item $a < b^d \rightarrow T(n) = \Theta(n^d)$
\end{itemize}

\section{Masters}
\begin{align*}
	T(n) &= aT(\frac{n}{b})+f(n) \\
	a &\geq 1 \\
	b &> 1
\end{align*}
\begin{itemize}
	\item $f(n) = \mathcal{O}(n^{log_ba-\epsilon})\rightarrow T(n) = \Theta(n^{\log_ba}), \epsilon > 0$
	\item $f(n) = \Theta(n^{log_ba})\rightarrow T(n) = \Theta(n^{log_ba}\log(n))$
	\item $f(n) = \Omega(n^{log_ba+\epsilon})\rightarrow T(n) = \Theta(f(n)), \epsilon > 0$
		and $af(\frac{n}{b}) \leq cf(n)$ for some $c < 1$ and big enough $n$
	\item case2 ext: $f(n) = \Theta(n^{log_ba}log^k(n)) \rightarrow T(n) = \Theta(n^{log_ba}log^{k+1}(n))$
\end{itemize}


\section{Akra-Bazzi}
\[
	T(n) = \sum_{i=1}^ka_iT(b_in)+f(n), n > n_0
\]
\begin{itemize}
	\item $n_0 \geq \frac{1}{b_i}$, $n_0 \geq \frac{1}{1-b_i}$ for each $i$,
	\item $a_i > 0$ for each $i$,
	\item $0<b_i$ for each $i$,
	\item $k \geq 1$,
	\item $f(n)$ is non-negative function,
	\item $c_1f(n) \leq f(u) \leq c_2f(n)$, for each $u$ satisfying condition: $b_in\leq u\leq n$
\end{itemize}
\[
	T(n) = \Theta(n^p(1+\int_1^n\frac{f(u)}{u^{p+1}}du))
\]
we get $p$ from:
\[
	\sum_{i=1}^ka_ib_i^p=1
\]
\subsection{Extended Akra-Bazzi}
\[
	T(n) = \sum_{i=1}^ka_iT(b_in+h_i(n))+f(n), n > n_0
\]
all of the conditions from Akra-Bazzi still hold plus:
\[
	|h_i(n)| = \mathcal{O}(\frac{n}{\log^2n})
\]

\section{Annihilators}
Steps:
\begin{itemize}
	\item Write the recurrence in operator form.
	\item Extract the annihilator for the recurrence.
	\item Factor the annihilator (if necessary).
	\item Extract the generic solution form the annihilator.
	\item Solve for coefficients using base cases (if known).
\end{itemize}
\setlength{\tabcolsep}{0.5em}{\renewcommand{\arraystretch}{1.2}
\begin{tabular}{ | c | c | }
    \hline
    \textbf{Operator} & \textbf{Definition}\\\hline
    addition & $(f+g)(n) := f(n)+g(n)$ \\
    subtraction & $(f-g)(n) := f(n)-g(n)$ \\
    multiplication & $(a\cdot f)(n) := a\cdot (f(n))$ \\
    shift & $E f(n) := f(n+1)$ \\
    $k$-fold shift & $E^k f(n) := f(n+k)$ \\ \hline
    composition & $(X+Y)f:= Xf+Yf$ \\
    & $(X-Y)f:= Xf-Yf$ \\
    & $XYf:= X(Yf)=Y(Xf)$ \\
    distribution & $X(f+g)= Xf+Xg$ \\\hline
\end{tabular}
}
\setlength{\tabcolsep}{0.5em}{\renewcommand{\arraystretch}{1.2}
\begin{tabular}{ | c | l | }
    \hline
    \textbf{Operator} & \textbf{Functions annihilated}\\\hline
    $E -1$ & $\alpha$ \\
    $E -a$ & $\alpha a^n$ \\
    $(E-a)(E-b)$ & $\alpha a^n+\beta b^n$\hfill (if $a \neq b$) \\
    $(E-a_0)(E-a_1)\cdots(E-a_k)$ & $\sum_{i=0}^k\alpha_ia_i^n$\hfill (if $a_i$ distinct) \\
    $(E - 1)^2$ & $\alpha n + \beta$ \\
    $(E - a)^2$ & $(\alpha n + \beta)a^n$ \\
    $(E - a)^2(E-b)$ & $(\alpha n + \beta)a^n+\gamma b^n$\hfill (if $a\neq b$)\\
    $(E - a)^d$ & $(\sum_{i=0}^{d-1}\alpha_in^i)a^n$ \\\hline\hline
    \multicolumn{2}{|c|}{If $X$ annihilates $f$, then $X$ also annihilates $E f$.} \\
    \multicolumn{2}{|c|}{If $X$ annihilates both $f$ and $g$, then $X$ also annihilates $f\pm g$.} \\
    \multicolumn{2}{|c|}{If $X$ annihilates $f$, then $X$ also annihilates $\alpha f$, for any constant $\alpha$.} \\\hline\hline
    \multicolumn{2}{|c|}{If $X$ annihilates $f$ and $Y$ annihilates $g$, then $XY$ annihilates $f\pm g$.} \\\hline
\end{tabular}
}

\end{multicols}
\end{document}
